define invariant saying that the cache only stores SLL target results, and prove some initial properties about it

SLL_Prediction.v
@@ -185,7 +185,7 @@ Module SllPredictionFn (Import D : Defs.T).
   Definition mkGraph (g : grammar) : closure_map :=
     fromEdges (mkGraphEdges g).
 
-  Definition callSites (cm : closure_map) (fr : suffix_frame) : list suffix_frame :=
+  Definition destFrames (cm : closure_map) (fr : suffix_frame) : list suffix_frame :=
     match FM.find fr cm with
     | Some s => FS.elements s
     | None   => []
@@ -193,245 +193,222 @@ Module SllPredictionFn (Import D : Defs.T).
 
   (* Now for the parts that correspond to the LL prediction module *)
 
-  (* "SLL closure" operation *)
-
-  Definition sllClosureStep (g  : grammar)
-                           (cm : closure_map)
-                           (av : NtSet.t)
-                           (sp : subparser) : subparser_closure_step_result :=
+  Definition simReturn (cm : closure_map) (sp : subparser) : option (list subparser) :=
     match sp with
-    | Sp pred (fr, frs) =>
-      match fr with
-      | SF o [] =>
-        match frs with
-        | [] =>
-          (* SLL-specific part -- simulate a return to all call sites *)
-          match o with
-          | None   => CstepDone [sp] (* maybe this is an error? *)
-          | Some x =>
-            let sps' := map (fun fr' => Sp pred (fr', [])) (callSites cm fr)
-            in  CstepDone sps'
-          end
-        | SF _ [] :: _                       => CstepError SpInvalidState
-        | SF _ (T _ :: _) :: _               => CstepError SpInvalidState
-        | SF o_cr (NT x :: suf_cr) :: frs_tl =>
-          let stk':= (SF o_cr suf_cr, frs_tl) 
-          in  CstepK (NtSet.add x av) [Sp pred stk'] 
-        end
-      | SF _ (T _ :: _)    => CstepDone [sp]
-      | SF _ (NT x :: suf) =>
-        if NtSet.mem x av then
-          let sps' := map (fun rhs => Sp pred 
-                                         (SF (Some x) rhs, fr :: frs))
-                          (rhssForNt g x)
-          in  CstepK (NtSet.remove x av) sps' 
-        else if NtSet.mem x (allNts g) then
-               CstepError (SpLeftRecursion x)
-             else
-               CstepK NtSet.empty [] 
-      end
+    | Sp pred (SF (Some x) [], []) =>
+      let dsts := destFrames cm (SF (Some x) []) in
+      let sps' := map (fun d => Sp pred (d, [])) dsts
+      in  Some sps'
+    | _ => None
     end.
 
-  Lemma sll_cstep_done_eq_or_map_lookup :
-    forall g cm av sp pr fr frs sps,
-      sp = Sp pr (fr, frs)
-      -> sllClosureStep g cm av sp = CstepDone sps
-      -> sps = [sp] \/ sps = map (fun fr' => Sp pr (fr', [])) (callSites cm fr).
+  Lemma simReturn_preserves_prediction :
+    forall cm sp sp' sps',
+      simReturn cm sp = Some sps'
+      -> In sp' sps'
+      -> prediction sp' = prediction sp.
   Proof.
-    intros g cm av sp pr fr frs sps ? hs; subst.
-    unfold sllClosureStep in hs; dms; tc; inv hs; auto.
+    intros cm [pred (fr, frs)] sp' sps' hs hi; sis; dms; tc; inv hs.
+    apply in_map_iff in hi; destruct hi as [? [? ?]]; subst; auto.
   Qed.
   
-  Lemma CstepK_sll_equiv_ll :
-    forall (g      : grammar)
-           (cm     : closure_map)
-           (sp sp' : subparser)
-           (sps'   : list subparser)
-           (av av' : NtSet.t),
-      sllClosureStep g cm av sp = CstepK av' sps'
-      -> spClosureStep g av sp = CstepK av' sps'.
-  Proof.
-    intros g cm sp sp' sps' av av' hs; unfold sllClosureStep in hs; dms; tc.
-  Defined.
-
-  Lemma acc_after_sll_step :
-    forall g cm sp sp' sps' av av',
-      sllClosureStep g cm av sp = CstepK av' sps'
-      -> In sp' sps'
-      -> Acc lex_nat_pair (meas g av sp)
-      -> Acc lex_nat_pair (meas g av' sp').
-  Proof.
-    intros g cm sp sp' sps' av av' heq hi ha.
-    eapply Acc_inv; eauto.
-    eapply spClosureStep_meas_lt; eauto.
-    eapply CstepK_sll_equiv_ll; eauto.
-  Defined.
-
-  Definition closure_result := sum prediction_error (list subparser).
-
-  Fixpoint sllSpClosure (g  : grammar)
-                        (cm : closure_map)
-                        (av : NtSet.t)
-                        (sp : subparser)
-                        (a  : Acc lex_nat_pair (meas g av sp))
-                        : closure_result :=
-    match sllClosureStep g cm av sp as r return sllClosureStep g cm av sp = r -> _ with
-    | CstepDone sps'  => fun _  => inr sps'
-    | CstepError e    => fun _  => inl e
-    | CstepK av' sps' => 
-      fun hs => 
-        let crs :=
-            dmap sps' (fun sp' hin =>
-                         sllSpClosure g cm av' sp'
-                                      (acc_after_sll_step _ _ _ _ _ _ _ hs hin a))
-        in  aggrClosureResults crs
-    end eq_refl.
-
-  Lemma sllSpClosure_unfold :
-    forall g cm av sp a,
-      sllSpClosure g cm av sp a =
-      match sllClosureStep g cm av sp as r return sllClosureStep g cm av sp = r -> _ with
-      | CstepDone sps'  => fun _  => inr sps'
+  Fixpoint sllc' (g  : grammar)
+                 (cm : closure_map)
+                 (av : NtSet.t)
+                 (sp : subparser)
+                 (a  : Acc lex_nat_pair (meas g av sp))
+    : closure_result :=
+    match simReturn cm sp with
+    | Some sps' => inr sps'
+    | None      =>
+      match spClosureStep g av sp as r return spClosureStep g av sp = r -> _ with
+      | CstepDone       => fun _  => inr [sp]
       | CstepError e    => fun _  => inl e
       | CstepK av' sps' => 
         fun hs => 
-          let crs := 
-              dmap sps' (fun sp' hin =>
-                           sllSpClosure g cm av' sp' (acc_after_sll_step _ _ _ _ _ _ _ hs hin a))
+          let crs := dmap sps' (fun sp' hin =>
+                                  sllc' g cm av' sp'
+                                            (acc_after_step _ _ _ _ hs hin a))
           in  aggrClosureResults crs
-      end eq_refl.
+      end eq_refl
+    end.
+
+  Lemma sllc'_unfold :
+    forall g cm av sp a,
+      sllc' g cm av sp a =
+      match simReturn cm sp with
+      | Some sps' => inr sps'
+      | None      =>
+        match spClosureStep g av sp as r return spClosureStep g av sp = r -> _ with
+        | CstepDone       => fun _  => inr [sp]
+        | CstepError e    => fun _  => inl e
+        | CstepK av' sps' => 
+          fun hs => 
+            let crs := dmap sps' (fun sp' hin =>
+                                    sllc' g cm av' sp'
+                                          (acc_after_step _ _ _ _ hs hin a))
+            in  aggrClosureResults crs
+        end eq_refl
+      end.
   Proof.
     intros g cm av sp a; destruct a; auto. 
   Qed.
-  
-  Lemma sllSpClosure_cases' :
+
+  Lemma sllc'_cases' :
     forall (g   : grammar)
            (cm  : closure_map)
-           (sp  : subparser)
            (av  : NtSet.t)
+           (sp  : subparser)
            (a   : Acc lex_nat_pair (meas g av sp))
            (sr  : subparser_closure_step_result)
            (cr  : closure_result)
-           (heq : sllClosureStep g cm av sp = sr),
-      match sr as r return sllClosureStep g cm av sp = r -> closure_result with
-      | CstepDone sps'  => fun _  => inr sps'
-      | CstepError e    => fun _  => inl e
-      | CstepK av' sps' => 
-        fun hs => 
-          let crs := dmap sps' (fun sp' hin => sllSpClosure g cm av' sp'
-                                                            (acc_after_sll_step _ _ _ _ _ _ _ hs hin a))
-          in  aggrClosureResults crs
-      end heq = cr
+           (heq : spClosureStep g av sp = sr),
+      match simReturn cm sp with
+      | Some sps' => inr sps'
+      | None      =>
+        match sr as r return spClosureStep g av sp = r -> closure_result with
+        | CstepDone       => fun _  => inr [sp]
+        | CstepError e    => fun _  => inl e
+        | CstepK av' sps' => 
+          fun hs => 
+            let crs := dmap sps' (fun sp' hin => sllc' g cm av' sp'
+                                                       (acc_after_step _ _ _ _ hs hin a))
+            in  aggrClosureResults crs
+        end heq
+      end = cr
       -> match cr with
          | inl e => 
            sr = CstepError e
            \/ exists (sps : list subparser)
                      (av' : NtSet.t)
-                     (hs  : sllClosureStep g cm av sp = CstepK av' sps)
+                     (hs  : spClosureStep g av sp = CstepK av' sps)
                      (crs : list closure_result),
                crs = dmap sps (fun sp' hi => 
-                                 sllSpClosure g cm av' sp'
-                                              (acc_after_sll_step _ _ _ _ _ _ _ hs hi a))
+                                 sllc' g cm av' sp'
+                                       (acc_after_step _ _ _ _ hs hi a))
                /\ aggrClosureResults crs = inl e
          | inr sps =>
-           match sp with
-           | Sp pred (fr, frs) =>
-             (sr = CstepDone sps
-              /\ (sps = [sp] \/ sps = map (fun fr' => Sp pred (fr', [])) (callSites cm fr)))
-             \/ exists (sps' : list subparser)
-                       (av'  : NtSet.t)
-                       (hs   : sllClosureStep g cm av sp = CstepK av' sps')
-                       (crs  : list closure_result),
-                 crs = dmap sps' (fun sp' hi => 
-                                    sllSpClosure g cm av' sp'
-                                                 (acc_after_sll_step _ _ _ _ _ _ _ hs hi a))
-                 /\ aggrClosureResults crs = inr sps
-           end
+           simReturn cm sp = Some sps
+           \/ (sr = CstepDone /\ sps = [sp])
+           \/ exists (sps' : list subparser)
+                     (av'  : NtSet.t)
+                     (hs   : spClosureStep g av sp = CstepK av' sps')
+                     (crs  : list closure_result),
+               crs = dmap sps' (fun sp' hi => 
+                                  sllc' g cm av' sp'
+                                        (acc_after_step _ _ _ _ hs hi a))
+               /\ aggrClosureResults crs = inr sps
          end.
   Proof.
-    intros g cm [pr (fr, frs)] av a sr cr heq.
-    destruct sr as [| sps | e];
-      destruct cr as [e' | sps']; intros heq'; tc;
-        try solve [inv heq'; eauto | eauto 8].
-    eapply sll_cstep_done_eq_or_map_lookup in heq; inv heq'; eauto.
+    intros g cm av sp a sr cr heq.
+    dms; tc; intros heq'; try solve [inv heq'; eauto | eauto 8].
   Qed.
   
-  Lemma sllSpClosure_cases :
+  Lemma sllc'_cases :
     forall (g  : grammar)
            (cm : closure_map)
            (sp : subparser)
            (av : NtSet.t)
            (a  : Acc lex_nat_pair (meas g av sp))
            (cr : closure_result),
-      sllSpClosure g cm av sp a = cr
+      sllc' g cm av sp a = cr
       -> match cr with
          | inl e => 
-           sllClosureStep g cm av sp = CstepError e
+           spClosureStep g av sp = CstepError e
            \/ exists (sps : list subparser)
                      (av' : NtSet.t)
-                     (hs  : sllClosureStep g cm av sp = CstepK av' sps)
+                     (hs  : spClosureStep g av sp = CstepK av' sps)
                      (crs : list closure_result),
                crs = dmap sps (fun sp' hi => 
-                                 sllSpClosure g cm av' sp'
-                                   (acc_after_sll_step _ _ _ _ _ _ _ hs hi a))
+                                 sllc' g cm av' sp'
+                                   (acc_after_step _ _ _ _ hs hi a))
                /\ aggrClosureResults crs = inl e
          | inr sps =>
-           match sp with
-           | Sp pred (fr, frs) =>
-             (sllClosureStep g cm av sp = CstepDone sps
-              /\ (sps = [sp]
-                  \/ sps = map (fun fr' => Sp pred (fr', [])) (callSites cm fr)))
-             \/ exists (sps' : list subparser)
-                       (av'  : NtSet.t)
-                       (hs   : sllClosureStep g cm av sp = CstepK av' sps')
-                       (crs  : list closure_result),
-                 crs = dmap sps' (fun sp' hi => 
-                                    sllSpClosure g cm av' sp'
-                                      (acc_after_sll_step _ _ _ _ _ _ _ hs hi a))
-                 /\ aggrClosureResults crs = inr sps
-           end
-         end.
+           simReturn cm sp = Some sps
+           \/ (spClosureStep g av sp = CstepDone /\ sps = [sp])
+           \/ exists (sps' : list subparser)
+                     (av'  : NtSet.t)
+                     (hs   : spClosureStep g av sp = CstepK av' sps')
+                     (crs  : list closure_result),
+               crs = dmap sps' (fun sp' hi => 
+                                  sllc' g cm av' sp'
+                                        (acc_after_step _ _ _ _ hs hi a))
+               /\ aggrClosureResults crs = inr sps
+           end.
   Proof.
     intros g cm av sp a cr hs; subst.
-    rewrite sllSpClosure_unfold.
-    eapply sllSpClosure_cases'; eauto.
+    rewrite sllc'_unfold.
+    eapply sllc'_cases'; eauto.
   Qed.
 
-  (*
-  Lemma spClosure_success_cases :
-    forall g sp av a sps,
-      spClosure g av sp a = inr sps
-      -> (spClosureStep g av sp = CstepDone sps /\ sps = [sp])
+  Lemma sllc'_success_cases :
+    forall g cm av sp a sps,
+      sllc' g cm av sp a = inr sps
+      -> simReturn cm sp = Some sps
+         \/ (spClosureStep g av sp = CstepDone /\ sps = [sp])
          \/ exists (sps' : list subparser)
                    (av'  : NtSet.t)
                    (hs   : spClosureStep g av sp = CstepK av' sps')
                    (crs  : list closure_result),
-          crs = dmap sps' (fun sp' hi => 
-                             spClosure g av' sp' (acc_after_step _ _ _ _ hs hi a))
-          /\ aggrClosureResults crs = inr sps.
+             crs = dmap sps' (fun sp' hi => 
+                                sllc' g cm av' sp'
+                                      (acc_after_step _ _ _ _ hs hi a))
+             /\ aggrClosureResults crs = inr sps.
   Proof.
-    intros g sp av a sps hs; apply spClosure_cases with (cr := inr sps); auto.
+    intros g cm av sp a sps hs; apply sllc'_cases with (cr := inr sps); auto.
   Qed.
 
-  Lemma spClosure_error_cases :
-    forall g sp av a e,
-      spClosure g av sp a = inl e
+  Lemma sllc'_error_cases :
+    forall g cm sp av a e,
+      sllc' g cm av sp a = inl e
       -> spClosureStep g av sp = CstepError e
          \/ exists (sps : list subparser)
                    (av' : NtSet.t)
                    (hs  : spClosureStep g av sp = CstepK av' sps)
                    (crs : list closure_result),
           crs = dmap sps (fun sp' hi => 
-                            spClosure g av' sp' (acc_after_step _ _ _ _ hs hi a))
+                            sllc' g cm av' sp' (acc_after_step _ _ _ _ hs hi a))
           /\ aggrClosureResults crs = inl e.
   Proof.
-    intros g sp av a e hs; apply spClosure_cases with (cr := inl e); auto.
+    intros g cm sp av a e hs; apply sllc'_cases with (cr := inl e); auto.
   Qed.
-   *)
+
+    Lemma sllc'_preserves_prediction' :
+    forall g cm pair (a : Acc lex_nat_pair pair) av sp sp' sps' a',
+      pair = meas g av sp
+      -> sllc' g cm av sp a' = inr sps'
+      -> In sp' sps'
+      -> sp'.(prediction) = sp.(prediction).
+  Proof.
+    intros g cm pair a.
+    induction a as [pair hlt IH]; intros av sp sp' sps' a' heq hs hi; subst.
+    apply sllc'_success_cases in hs.
+    destruct hs as [hs | [[hs heq] | [sps'' [av' [hs [crs [heq heq']]]]]]]; subst.
+    - eapply simReturn_preserves_prediction; eauto. 
+    - apply in_singleton_eq in hi; subst; auto.
+    - (* lemma *)
+      eapply aggrClosureResults_succ_in_input in heq'; eauto.
+      destruct heq' as [sps [hi' hi'']].
+      eapply dmap_in in hi'; eauto.
+      destruct hi' as [sp'' [hi''' [_ heq]]].
+      eapply IH in heq; subst; eauto.
+      + apply spClosureStep_preserves_prediction with (sp' := sp'') in hs; auto.
+        rewrite hs; auto.
+      + eapply spClosureStep_meas_lt; eauto.
+  Qed.
+
+  Lemma sllc'_preserves_prediction :
+    forall g cm av sp sp' sps' (a : Acc lex_nat_pair (meas g av sp)),
+      sllc' g cm av sp a = inr sps'
+      -> In sp' sps'
+      -> sp'.(prediction) = sp.(prediction).
+  Proof.
+    intros; eapply sllc'_preserves_prediction'; eauto.
+  Qed.
   
   Definition sllClosure (g : grammar) (cm : closure_map) (sps : list subparser) :
     sum prediction_error (list subparser) :=
-    aggrClosureResults (map (fun sp => sllSpClosure g cm (allNts g) sp (lex_nat_pair_wf _)) sps).
+    aggrClosureResults (map (fun sp => sllc' g cm (allNts g) sp (lex_nat_pair_wf _)) sps).
 
   Lemma sllClosure_preserves_prediction :
     forall g cm sps sp' sps',
@@ -439,7 +416,13 @@ Module SllPredictionFn (Import D : Defs.T).
       -> In sp' sps'
       -> exists sp, In sp sps /\ prediction sp' = prediction sp.
   Proof.
-  Admitted.
+    intros g cm sps sp' sps' hc hi.
+    eapply aggrClosureResults_succ_in_input in hc; eauto.
+    destruct hc as [sps'' [hi' hi'']].
+    apply in_map_iff in hi'; destruct hi' as [sp [hspc hi''']].
+    eexists; split; eauto.
+    eapply sllc'_preserves_prediction; eauto.
+  Qed.
 
   (* SLL prediction *)
 
@@ -466,14 +449,36 @@ Module SllPredictionFn (Import D : Defs.T).
 
   Definition empty_cache : cache := Cache.empty (list subparser).
 
-  Definition target g cm (sps : list subparser) (a : terminal) : sum prediction_error (list subparser) :=
+  Definition sllTarget g cm (sps : list subparser) (a : terminal) : sum prediction_error (list subparser) :=
     match move a sps with
-    | inl e => inl e
-    | inr sps' => match sllClosure g cm sps' with
-                  | inl e => inl e
-                  | inr sps'' => inr sps''
-                  end
+    | inl e    => inl e
+    | inr sps' =>
+      match sllClosure g cm sps' with
+      | inl e => inl e
+      | inr sps'' => inr sps''
+      end
     end.
+
+  Lemma sllTarget_preserves_prediction :
+    forall g cm sps a sp' sps',
+      sllTarget g cm sps a = inr sps'
+      -> In sp' sps'
+      -> exists sp, In sp sps /\ prediction sp = prediction sp'.
+  Proof.
+    intros g cm sps a sp' sps'' hs hi.
+    unfold sllTarget in hs.
+    destruct (move _ _)         as [? | sps' ] eqn:hm; tc.
+    destruct (sllClosure _ _ _) as [? | ?    ] eqn:hc; tc; inv hs.
+    eapply sllClosure_preserves_prediction in hc; eauto.
+    destruct hc as [sp'' [hi'' heq]]; rewrite heq.
+    eapply move_preserves_prediction in hm; eauto.
+    destruct hm as [? [? ?]]; eauto.
+  Qed.
+
+  Definition cache_stores_target_results g ca cm :=
+    forall sps a sps',
+      Cache.find (sps, a) ca = Some sps'
+      -> sllTarget g cm sps a = inr sps'.
 
     (* To do: maybe only PredSucc and PredAmbig should carry an updated cache *)
   Fixpoint sllPredict' (g : grammar) (cm : closure_map) (sps : list subparser) (ts : list token) (c : cache) : prediction_result * cache :=
@@ -489,7 +494,7 @@ Module SllPredictionFn (Import D : Defs.T).
           match Cache.find (sps, a) c with 
           | Some sps' => sllPredict' g cm sps' ts' c
           | None      =>
-            match target g cm sps a with
+            match sllTarget g cm sps a with
             | inl e    => (PredError e, c)
             | inr sps' =>
               let c' := Cache.add (sps, a) sps' c
@@ -501,11 +506,12 @@ Module SllPredictionFn (Import D : Defs.T).
 
   Lemma sllPredict'_success_result_in_original_subparsers :
     forall g cm ts ca ca' ys sps,
-      sllPredict' g cm sps ts ca = (PredSucc ys, ca')
+      cache_stores_target_results g ca cm
+      -> sllPredict' g cm sps ts ca = (PredSucc ys, ca')
       -> exists sp, In sp sps /\ sp.(prediction) = ys.
   Proof.
     intros g cm ts. 
-    induction ts as [| (a,l) ts IH]; intros ca ca' ys sps hp; sis.
+    induction ts as [| (a,l) ts IH]; intros ca ca' ys sps hc hp; sis.
     - destruct sps as [| sp sps']; tc; dmeq hall.
       + inv hp; exists sp; split; auto.
         apply in_eq.
@@ -516,23 +522,35 @@ Module SllPredictionFn (Import D : Defs.T).
       + inv hp; exists sp; split; auto.
         apply in_eq.
       + dmeq hf; tc.
-        * (* need an invariant about the cache here *)
-          apply IH in hp; destruct hp as [sp' [hi heq]]; subst.
-          admit.
-        * (* to do : lemma about target function *)
-          unfold target in hp.
-          destruct (move _ _) as [m | sps''] eqn:hm; tc.
-          destruct (sllClosure _ _ _) as [m | sps'''] eqn:hc; tc.
-          apply IH in hp; destruct hp as [? [? ?]]; subst.
-          eapply sllClosure_preserves_prediction in hc; eauto.
-          destruct hc as [sp'' [hi'' heq]]; rewrite heq.
-          eapply move_preserves_prediction in hm; eauto.
-          destruct hm as [? [? ?]]; eauto.
-  Admitted.
+        * apply IH in hp; auto; destruct hp as [sp' [hi heq]]; subst.
+          apply hc in hf.
+          eapply sllTarget_preserves_prediction; eauto.
+        * dmeq ht; tc.
+          apply IH in hp.
+          -- destruct hp as [sp' [hi ?]]; subst.
+             eapply sllTarget_preserves_prediction; eauto.
+          -- (* lemma *)
+            red.
+            intros ss t ss' hfind.
+            destruct (cache_key_eq_dec (ss, t) (sp :: sps', a)).
+            ++ inv e.
+               rewrite CacheFacts.add_eq_o in hfind; auto.
+               inv hfind; auto.
+            ++ rewrite CacheFacts.add_neq_o in hfind; auto.
+  Qed.
   
   Definition sllInitSps (g : grammar) (x : nonterminal) : list subparser :=
     map (fun rhs => Sp rhs (SF (Some x) rhs, []))
         (rhssForNt g x).
+
+  Lemma sllInitSps_prediction_in_rhssForNt :
+    forall g x sp,
+      In sp (sllInitSps g x)
+      -> In sp.(prediction) (rhssForNt g x).
+  Proof.
+    intros g x sp hi; unfold sllInitSps in hi.
+    apply in_map_iff in hi; firstorder; subst; auto.
+  Qed.
 
   Definition sllStartState (g : grammar) (cm : closure_map)
              (x : nonterminal) : sum prediction_error (list subparser) :=
@@ -546,7 +564,10 @@ Module SllPredictionFn (Import D : Defs.T).
   Proof.
     intros g cm x sp' sps' hs hi.
     unfold sllStartState in hs.
-  Admitted.
+    eapply sllClosure_preserves_prediction in hs; eauto.
+    destruct hs as [sp [hi' heq]]; rewrite heq.
+    apply sllInitSps_prediction_in_rhssForNt; auto.
+  Qed.
 
   Definition sllPredict (g : grammar) (cm : closure_map) (x : nonterminal)
              (ts : list token) (c : cache) : prediction_result * cache :=
@@ -557,12 +578,13 @@ Module SllPredictionFn (Import D : Defs.T).
 
   Lemma sllPredict_succ_in_rhssForNt :
     forall g cm x ts ca ca' ys,
-      sllPredict g cm x ts ca = (PredSucc ys, ca')
+      cache_stores_target_results g ca cm
+      -> sllPredict g cm x ts ca = (PredSucc ys, ca')
       -> In ys (rhssForNt g x).
   Proof.
-    intros g cm x ts ca ca' ys hs; unfold sllPredict in hs.
+    intros g cm x ts ca ca' ys hc hs; unfold sllPredict in hs.
     dmeq hs'; tc.
-    eapply sllPredict'_success_result_in_original_subparsers in hs.
+    eapply sllPredict'_success_result_in_original_subparsers in hs; eauto.
     destruct hs as [sp [hi heq]]; subst.
     eapply sllStartState_sp_prediction_in_rhssForNt; eauto.
   Qed.
@@ -576,10 +598,11 @@ Module SllPredictionFn (Import D : Defs.T).
   
   Lemma adaptivePredict_succ_in_rhssForNt :
     forall g cm x ss ts ca ca' ys,
-      adaptivePredict g cm x ss ts ca = (PredSucc ys, ca')
+      cache_stores_target_results g ca cm
+      -> adaptivePredict g cm x ss ts ca = (PredSucc ys, ca')
       -> In ys (rhssForNt g x).
   Proof.
-    intros g cm x ss ts ca ca' ys ha.
+    intros g cm x ss ts ca ca' ys hc ha.
     unfold adaptivePredict in ha; dmeqs h; tc; inv ha.
     - eapply sllPredict_succ_in_rhssForNt; eauto.
     - eapply llPredict_succ_in_rhssForNt; eauto.
@@ -587,20 +610,22 @@ Module SllPredictionFn (Import D : Defs.T).
   
   Lemma adaptivePredict_succ_in_grammar :
     forall g cm x ss ts ca ca' ys,
-      adaptivePredict g cm x ss ts ca = (PredSucc ys, ca')
+      cache_stores_target_results g ca cm
+      -> adaptivePredict g cm x ss ts ca = (PredSucc ys, ca')
       -> In (x, ys) g.
   Proof.
-    intros g cm x ss ts ca ca' ys ha.
+    intros g cm x ss ts ca ca' ys hc ha.
     apply rhssForNt_in_iff.
     eapply adaptivePredict_succ_in_rhssForNt; eauto.
   Qed.
 
   Lemma adaptivePredict_ambig_in_grammar :
     forall g cm x ss ts ca ca' ys,
-      adaptivePredict g cm x ss ts ca = (PredAmbig ys, ca')
+      cache_stores_target_results g ca cm
+      -> adaptivePredict g cm x ss ts ca = (PredAmbig ys, ca')
       -> In (x, ys) g.
   Proof.
-    intros g cm x ss ts ca ca' ys ha.
+    intros g cm x ss ts ca ca' ys hc ha.
     unfold adaptivePredict in ha; dms; tc; inv ha.
     eapply llPredict_ambig_in_grammar; eauto.
   Qed.
